Finish TreeSet and move generic stuff to Sets

examples/SinglyLinkedList.v
@@ -64,12 +64,12 @@ End SinglyLinkedList.
 Import SinglyLinkedList.
 Hint Immediate sll_extensional.
 
-Definition hints_sll' : TacPackage.
+Definition hints' : TacPackage.
   prepare1 (nil_fwd, cons_fwd) (nil_bwd, cons_bwd).
 Defined.
 
-Definition hints_sll : TacPackage.
-  prepare2 hints_sll'.
+Definition hints : TacPackage.
+  prepare2 hints'.
 Defined.
 
 Definition null A (ls : list A) : bool :=
@@ -160,6 +160,6 @@ Ltac finish := repeat match goal with
 
 Theorem sllMOk : moduleOk sllM.
 (*TIME Clear Timing Profile. *)
-  vcgen; abstract (sep hints_sll; finish).
+  vcgen; abstract (sep hints; finish).
 (*TIME Print Timing Profile. *)
 Qed.
